start calendar example, renovating coq proofs

new_example/calendar.go
@@ -1,0 +1,21 @@
+package main
+
+import "github.com/tchajed/marshal"
+
+type Calendar struct {
+	events []Event
+}
+
+func MarshalCalendar(enc []byte, c Calendar) []byte {
+	enc = marshal.WriteInt(enc, uint64(len(c.events)))
+	return marshal.WriteSlice[Event](enc, c.events, MarshalEvent)
+}
+
+func UnmarshalCalendar(s []byte) (Calendar, []byte) {
+	eventsLen, s := marshal.ReadInt(s)
+	events, s := marshal.ReadSlice[Event](s, eventsLen, UnmarshalEvent)
+
+	return Calendar{
+		events: events,
+	}, s
+}
