testdata/out/coq/event_proof_gk.v
@@ -3,116 +3,44 @@
 (*    DO NOT MANUALLY EDIT THIS FILE     *)
 (*****************************************)
 
-From Perennial.program_proof Require Import grove_prelude.
-From Perennial.program_proof Require Import marshal_stateless_proof.
+From New.proof Require Import proof_prelude.
+From New.proof Require Import github_com.tchajed.marshal.
 From New.code Require Import github_com.mjschwenne.grackle.testdata.out.go.event_gk.
+From New.generatedproof Require Import github_com.mjschwenne.grackle.testdata.out.go.event_gk.
 From Grackle.test Require Import timestamp_proof_gk.
 From New.code Require Import github_com.mjschwenne.grackle.testdata.out.go.timestamp_gk.
-From Perennial.goose_lang Require Import lib.slice.pred_slice.
 
-Module Event.
-Section Event.
+Module Event_gk.
+Section Event_gk.
 
-Typeclasses Opaque app.
+Context `{hG: heapGS Σ, !ffi_semantics _ _}.
+Context `{!goGlobalsGS Σ}.
 
-Context `{!heapGS Σ}.
+#[global]
+Program Instance : IsPkgInit event_gk :=
+  ltac2:(build_pkg_init ()).
 
-Record C :=
-    mkC {
-        id :  u32;
-        name :  byte_string;
-        startTime :  TimeStamp.C;
-        endTime :  TimeStamp.C;
-        }.
-
-Definition has_encoding (encoded:list u8) (args:C) : Prop :=
+Definition has_encoding (encoded:list u8) (args:event_gk.Event.t) : Prop :=
   ∃ (startTime_enc endTime_enc : list u8), 
-  encoded = (u32_le args.(id)) ++
-              (u64_le $ length $ args.(name)) ++ args.(name) ++
+  encoded = (u32_le args.(event_gk.Event.id)) ++
+              (u64_le $ length $ args.(event_gk.Event.name')) ++ args.(event.Event.name') ++
               startTime_enc ++
               endTime_enc
-  /\ TimeStamp.has_encoding startTime_enc args.(startTime)
-  /\ TimeStamp.has_encoding endTime_enc args.(endTime).
+  /\ TimeStamp_gk.has_encoding startTime_enc args.(startTime)
+  /\ TimeStamp_gk.has_encoding endTime_enc args.(endTime).
 
-Definition own (args__v: val) (args__c: C) (dq: dfrac) : iProp Σ :=
-  ∃(startTime__v endTime__v : val) , 
-  "%Hown_struct" ∷ ⌜ args__v = (#args__c.(id), (#(str args__c.(name)), (startTime__v, (endTime__v, #()))))%V ⌝ ∗
-  "Hown_startTime" ∷ TimeStamp.own startTime__v args__c.(startTime) dq ∗
-  "Hown_endTime" ∷ TimeStamp.own endTime__v args__c.(endTime) dq.
-
-
-Definition to_val' (c : C) : val :=
-  (#c.(id), (#(str c.(name)), (TimeStamp.to_val' c.(startTime), (TimeStamp.to_val' c.(endTime), #())))).
-
-Definition from_val' (v : val) : option C :=
-  match v with
-  | (#(LitInt32 id), (#(LitString name), (startTime, (endTime, #()))))%V =>
-    match TimeStamp.from_val' startTime with
-    | Some startTime =>
-        match TimeStamp.from_val' endTime with
-        | Some endTime =>
-            Some (mkC id name startTime endTime)
-        | None => None
-        end
-    | None => None
-    end
-  | _ => None
-  end.
-
-#[global]
-Instance Event_into_val : IntoVal C.
-Proof.
-  refine {|
-    to_val := to_val';
-    from_val := from_val';
-    IntoVal_def := (mkC (W32 0) "" (IntoVal_def TimeStamp.C) (IntoVal_def TimeStamp.C))
-  |}.
-  intros v. 
-  destruct v as [id name [startTime_hour startTime_minute startTime_second] [endTime_hour endTime_minute endTime_second]]; done.
-Defined.
-
-#[global]
-Instance Event_into_val_for_type : IntoValForType C (struct.t event_gk.S).
-Proof. constructor; auto 10. Defined.
-
-Lemma own_to_val (v : val) (c : C) (dq : dfrac) :
-  own v c dq -∗ ⌜ v = to_val c ⌝.
-Proof.
-  iIntros "Hown". iNamed "Hown".
-  
-  iDestruct (TimeStamp.own_to_val with "Hown_startTime") as "%Hval_startTime".
-  
-  iDestruct (TimeStamp.own_to_val with "Hown_endTime") as "%Hval_endTime".
-  
-  subst. done.
-Qed.
-
-
-Lemma own_val_ty :
-  ∀ (v : val) (x : C) (dq : dfrac), own v x dq -∗ ⌜val_ty v (struct.t event_gk.S)⌝.
-Proof.
-  iIntros (???) "Hown".
-  unfold own. iNamed "Hown".
-  
-  unfold timestamp_proof_gk.TimeStamp.own.
-  iNamed "Hown_startTime".
-  iNamed "Hown_endTime".
-  iPureIntro.
-  subst.
-  repeat constructor.
-Qed.
-
-Lemma wp_Encode (args__v : val) (args__c : C) (pre_sl : Slice.t) (prefix : list u8) (dq : dfrac):
+Lemma wp_Encode (args__c : event_gk.Event.t) (pre_sl : slice.t) (prefix : list u8) (dq : dfrac):
   {{{
-        own args__v args__c dq ∗
-        own_slice pre_sl byteT (DfracOwn 1) prefix
+        is_pkg_init event_gk ∗
+        own_slice pre_sl (DfracOwn 1) prefix ∗
+        own_slice_cap w8 pre_sl
   }}}
-    event_gk.Marshal (slice_val pre_sl) args__v
+    event_gk @ "Marshal" #pre_sl #args__c
   {{{
-        enc enc_sl, RET (slice_val enc_sl);
+        enc enc_sl, RET #enc_sl;
         ⌜ has_encoding enc args__c ⌝ ∗
-        own args__v args__c dq ∗
-        own_slice enc_sl byteT (DfracOwn 1) (prefix ++ enc)
+        own_slice enc_sl (DfracOwn 1) (prefix ++ enc) ∗
+        own_slice_cap w8 enc_sl
   }}}.
 
 Proof.
@@ -157,16 +85,16 @@ Proof.
   } done.
 Qed.
 
-Lemma wp_Decode (enc : list u8) (enc_sl : Slice.t) (args__c : C) (suffix : list u8) (dq : dfrac):
+Lemma wp_Decode (enc : list u8) (enc_sl : slice.t) (args__c : event_gk.Event.t) (suffix : list u8) (dq : dfrac):
   {{{
+        is_pkg_init event_gk ∗
         ⌜ has_encoding enc args__c ⌝ ∗
-        own_slice_small enc_sl byteT dq (enc ++ suffix)
+        own_slice enc_sl dq (enc ++ suffix)
   }}}
-    event_gk.Unmarshal (slice_val enc_sl)
+    event_gk @ "Unmarshal" #enc_sl
   {{{
-        args__v suff_sl, RET (args__v, suff_sl);
-        own args__v args__c (DfracOwn 1) ∗
-        own_slice_small suff_sl byteT dq suffix
+        suff_sl, RET (#args__c, suff_sl);
+        own_slice suff_sl dq suffix
   }}}.
 
 Proof.
@@ -223,6 +151,6 @@ Proof.
   iPureIntro. reflexivity.
 Qed.
 
-End Event.
-End Event.
+End Event_gk.
+End Event_gk.
 
