new_example/calendar_proof.v
@@ -1,0 +1,43 @@
+From New.proof Require Import proof_prelude.
+From Grackle.new_ex Require Import goose.github_com.mjschwenne.grackle.new_example.
+From Grackle.new_ex Require Import pg.github_com.mjschwenne.grackle.new_example.
+From New.proof Require Import github_com.tchajed.marshal.
+From Grackle.new_ex Require Import event_proof.
+
+Module Calendar_Proof.
+  Section Calendar_Proof.
+
+    Context `{hG: heapGS Σ, !ffi_semantics _ _}.
+    Context `{!goGlobalsGS Σ}.
+
+    #[global]
+      Program Instance : IsPkgInit main :=
+        ltac2:(build_pkg_init ()).
+
+    (* TODO: Figure out the impacts of not having pred_slice ported. *)
+    Definition has_encoding (encoded:list u8) (args:main.Calendar.t) : Prop :=
+      ∃ (events : list main.Event.t) (events__enc : list u8),
+        encoded = (u64_le $ args.(main.Calendar.events').(slice.len_f)) ++ events__enc /\
+        encodes events__enc events Event_Proof.has_encoding /\
+        length events < 2^64.
+
+    Lemma wp_Encode (args__c:main.Calendar.t) (pre_sl:slice.t) (prefix:list u8) (dq:dfrac):
+      uint.nat args__c.(main.Calendar.events').(slice.len_f) < 2^64 ->
+      {{{
+            is_pkg_init main ∗
+            own_slice pre_sl (DfracOwn 1) prefix ∗
+            own_slice_cap w8 pre_sl 
+      }}}
+        main @ "MarshalCalendar" #pre_sl #args__c
+      {{{
+            enc enc_sl, RET #enc_sl;
+            ⌜ has_encoding enc args__c ⌝ ∗
+            own_slice enc_sl (DfracOwn 1) (prefix ++ enc) ∗
+            own_slice_cap w8 enc_sl
+      }}}.
+
+      Proof.
+      Admitted.
+  End Calendar_Proof.
+End Calendar_Proof.
+    
